doc-src/TutorialI/Types/Overloading.thy
@@ -4,8 +4,9 @@ by intro_classes
 
 text{*\noindent
 This \isacommand{instance} declaration can be read like the declaration of
-a function on types: the constructor @{text list} maps types of class @{text
-term}, i.e.\ all HOL types, to types of class @{text ordrel}, i.e.\
+a function on types.  The constructor @{text list} maps types of class @{text
+term} (all HOL types), to types of class @{text ordrel};
+in other words,
 if @{text"ty :: term"} then @{text"ty list :: ordrel"}.
 Of course we should also define the meaning of @{text <<=} and
 @{text <<} on lists:
